Fix building, dependency cycle

disk-betree/Framework.cs
@@ -469,38 +469,6 @@ namespace Native_Compile {
 
           //Native_Compile.BenchmarkingUtil.end();
       }
-
-      [DllImport("c", CallingConvention = CallingConvention.Cdecl)]
-      private static extern unsafe int memcmp(byte* b1, byte* b2, int count);
-
-      public static int @ByteSeqCmpByteSeq(
-        Dafny.Sequence<byte> s1,
-        Dafny.Sequence<byte> s2)
-      {
-        var seg1 = (ArraySegment<int>) s1.Elements;
-        var seg2 = (ArraySegment<int>) s2.Elements;
-
-        int result;
-        unsafe {
-          fixed (byte* b1 = seg1.Array) {
-            fixed (byte* b2 = seg2.Array) {
-              result = memcmp(b1 + seg1.Offset, b2 + seg2.Offset, Math.Min(seg1.Count, seg2.Count));
-            }
-          }
-        }
-
-        if (result < 0) {
-          return -1;
-        } else if (result > 0) {
-          return 1;
-        } else if (seg1.Count < seg2.Count) {
-          return -1;
-        } else if (seg1.Count > seg2.Count) {
-          return 1;
-        } else {
-          return 0;
-        }
-      }
   }
 }
 
@@ -552,5 +520,42 @@ namespace Crypto_Compile {
     {
       return padded_crc32(ar, (int)start, (int)len);
     }
+  }
+}
+
+namespace TotalOrderNative_Compile {
+  public partial class @Arrays
+  {
+      [DllImport("c", CallingConvention = CallingConvention.Cdecl)]
+      private static extern unsafe int memcmp(byte* b1, byte* b2, int count);
+
+      public static int @ByteSeqCmpByteSeq(
+        Dafny.Sequence<byte> s1,
+        Dafny.Sequence<byte> s2)
+      {
+        var seg1 = (ArraySegment<byte>) s1.Elements;
+        var seg2 = (ArraySegment<byte>) s2.Elements;
+
+        int result;
+        unsafe {
+          fixed (byte* b1 = seg1.Array) {
+            fixed (byte* b2 = seg2.Array) {
+              result = memcmp(b1 + seg1.Offset, b2 + seg2.Offset, Math.Min(seg1.Count, seg2.Count));
+            }
+          }
+        }
+
+        if (result < 0) {
+          return -1;
+        } else if (result > 0) {
+          return 1;
+        } else if (seg1.Count < seg2.Count) {
+          return -1;
+        } else if (seg1.Count > seg2.Count) {
+          return 1;
+        } else {
+          return 0;
+        }
+      }
   }
 }
