lib/Marshalling/Native.s.dfy
@@ -26,22 +26,6 @@ module {:extern} Native {
           ensures  forall i :: (srcIndex as int) <= i < (srcIndex as int) + (len as int) ==>
                       src[i] == dst[i - (srcIndex as int) + (dstIndex as int)];
 
-      static predicate lt(a: seq<byte>, b: seq<byte>)
-      {
-        if |a| == 0 && |b| == 0 then false
-        else if |a| == 0 then true
-        else if |b| == 0 then false
-        else if a[0] < b[0] then true
-        else if a[0] > b[0] then false
-        else lt(a[1..], b[1..])
-      }
-
-      static method{:axiom} ByteSeqCmpByteSeq(s1: seq<byte>, s2: seq<byte>)
-          returns (c : int32)
-          ensures c < 0 ==> lt(s1, s2)
-          ensures c > 0 ==> lt(s2, s1)
-          ensures c == 0 ==> s1 == s2
-
   }
 
   class BenchmarkingUtil {
